src/Language/PlutusIR/Semantics/SemanticEquivalence/CompatibilityLemmas/Constant.v
@@ -2,7 +2,6 @@ Require Import PlutusCert.Language.PlutusIR.
 Import NamedTerm.
 Require Import PlutusCert.Language.PlutusIR.Semantics.Dynamic.
 Require Import PlutusCert.Language.PlutusIR.Semantics.Static.
-Require Import PlutusCert.Language.PlutusIR.Semantics.Static.Implementations.Named.
 Require Import PlutusCert.Language.PlutusIR.Semantics.SemanticEquivalence.LogicalRelation.RelationalModel.
 
 Require Import Arith.
