src/Language/PlutusIR/Semantics/SemanticEquivalence/LogicalRelation/TypeSubstitution.v
@@ -1,0 +1,99 @@
+Require Import PlutusCert.Language.PlutusIR.
+Import NamedTerm.
+Require Import PlutusCert.Language.PlutusIR.Semantics.Dynamic.
+Require Import PlutusCert.Language.PlutusIR.Semantics.Static.
+Require Import PlutusCert.Language.PlutusIR.Semantics.SemanticEquivalence.LogicalRelation.RelationalModel.
+
+
+Fixpoint map_msubstT_rho_syn1 (rho : tymapping) (xts : tass) : tass :=
+  match xts with
+  | nil => nil
+  | (x,T) :: xts' => (x, msubstT_rho_syn1 rho T) :: map_msubstT_rho_syn1 rho xts'
+  end.
+
+Fixpoint map_msubstT_rho_syn2 (rho : tymapping) (xts : tass) : tass :=
+  match xts with
+  | nil => nil
+  | (x,T) :: xts' => (x, msubstT_rho_syn2 rho T) :: map_msubstT_rho_syn2 rho xts'
+  end.
+
+Definition substituteT_context (a : tyname) (S : Ty) (Gamma : partial_map Ty) :=
+   fun x => 
+    match Gamma x with
+    | None => None
+    | Datatypes.Some T => 
+        Datatypes.Some (substituteT a S T)
+    end.
+
+
+
+(** ** Lemma C.6 *)
+
+(** *** Predicates *)
+
+Definition P_Term (e : Term) :=
+  forall a Gamma Delta T2 T1 K e_s,
+    (Gamma, a |-> K ; Delta) |-+ e : T2 ->
+    (Gamma, Delta) |-* T1 : K ->
+    annotsubst a T1 e e_s ->
+    (substituteT_context a T1 Gamma, Delta) |-+ e_s : (substituteT a T1 T2).
+
+Definition P_Binding (b : Binding) : Prop :=
+  forall ctx x U v b',
+    extendT x U ctx |-ok b ->
+    emptyContext |-+ v : U ->
+    substitute_binding x v b b' ->
+    ctx |-ok b' /\ binds b = binds b'.
+#[export] Hint Unfold P_Binding : core.
+
+Definition P_Bindings_NonRec (bs : list Binding) : Prop :=
+  forall ctx x U v bs',
+    extendT x U ctx |-oks_nr bs ->
+    emptyContext |-+ v : U ->
+    Util.ForallP P_Binding bs ->
+    substitute_bindings_nonrec x v bs bs' ->
+    ctx |-oks_nr bs' /\ List.map binds bs = List.map binds bs'.
+
+Definition P_Bindings_Rec (bs : list Binding) : Prop :=
+  forall ctx x U v bs',
+    extendT x U ctx |-oks_r bs ->
+    emptyContext |-+ v : U ->
+    Util.ForallP P_Binding bs ->
+    substitute_bindings_rec x v bs bs' ->
+    ctx |-oks_r bs' /\ List.map binds bs = List.map binds bs'.
+
+Lemma P_Bindings_NonRec__holds_definitionally : forall bs, P_Bindings_NonRec bs.
+Proof.
+Abort.
+
+Lemma P_Bindings_Rec__holds_definitionally : forall bs, P_Bindings_Rec bs.
+Proof.
+Abort.
+
+Axiom skip : forall P, P.
+
+Lemma type_substitution : forall e,
+    P_Term e.
+Proof.
+  apply Term__ind with P_Binding.
+  - apply skip.
+  - apply skip.
+  - (* T_TyAbs *)
+    intros bX K t IH__t.
+    unfold P_Term.
+    intros a Gamma Delta T2 T1 K0 e_s Htyp Hkind__T1 Has__e_s.
+    inversion Htyp. subst.
+    inversion Has__e_s.
+    + subst.
+      simpl.
+      rewrite eqb_refl.
+      apply T_TyAbs.
+      unfold P_Term in IH__t.
+      apply annotsubst_preserves_typing.
+      eapply IH__t.
+      unfold extendK in H4. fold extendK in H4.
+      eapply IH__t.
+      simpl.
+
+
+ Admitted.
