src/Language/PlutusIR/Semantics/SemanticEquivalence/Monotonicity.v
@@ -1,9 +1,8 @@
 Require Import PlutusCert.Language.PlutusIR.
 Import NamedTerm.
 Require Import PlutusCert.Language.PlutusIR.Semantics.Static.
-Require Import PlutusCert.Language.PlutusIR.Semantics.Static.Implementations.Named.
 Require Import PlutusCert.Language.PlutusIR.Semantics.Dynamic.
-Require Import PlutusCert.Language.PlutusIR.Semantics.SemanticEquivalence.Def.
+Require Import PlutusCert.Language.PlutusIR.Semantics.SemanticEquivalence.LogicalRelation.RelationalModel.
 
 Require Import Arith.
 
