src/Language/PlutusIR/Semantics/TypeSafety/AnnotsubstPreservesTyping.v
@@ -1,7 +1,6 @@
 Require Import PlutusCert.Language.PlutusIR.
 Import NamedTerm.
 Require Import PlutusCert.Language.PlutusIR.Semantics.Static.
-Require Import PlutusCert.Language.PlutusIR.Semantics.Static.Implementations.Named.
 Require Import PlutusCert.Language.PlutusIR.Semantics.Dynamic.Substitution.
 
 Theorem annotsubst_preserves_typing : forall Gamma X K U T t t',
