src/Language/PlutusIR/Semantics/TypeSafety/Preservation.v
@@ -1,9 +1,6 @@
 Require Import PlutusCert.Language.PlutusIR.
 Import NamedTerm.
 Require Import PlutusCert.Language.PlutusIR.Semantics.Static.
-Require Import PlutusCert.Language.PlutusIR.Semantics.Static.Implementations.Named.
-Require Import PlutusCert.Language.PlutusIR.Semantics.Static.Implementations.Named.ContextInvariance.
-Require Import PlutusCert.Language.PlutusIR.Semantics.Static.Implementations.Named.UniqueTypes.
 Require Import PlutusCert.Language.PlutusIR.Semantics.Dynamic.
 
 Require Import PlutusCert.Language.PlutusIR.Semantics.TypeSafety.SubstitutionPreservesTyping.
